theories/typechecker/typechecker.v
@@ -5186,56 +5186,10 @@ Proof.
 Qed.
 
 Lemma has_function_type_checker_correct :
-  ∀ M mf ft, has_function_type_checker M mf ft = ok_term ->
-             has_function_type M mf ft.
+  ∀ M mf, has_function_type_checker M mf mf.(mf_type) = ok_term ->
+          has_function_type M mf.
 Proof.
-  intros.
-  Opaque have_instruction_type_checker.
-  unfold has_function_type_checker in H.
-  repeat my_auto5.
-  rename l into ηss_L; rename l0 into ρs_P; rename l1 into ηss_P.
-  rename l2 into L'.
-  apply function_type_eq_convert in HMatch. subst ft.
-  apply (TFunction M mf ηss_L ηss_P ρs_P L'); auto.
-  - cbn. (* lemma: prove that grab rep with messed up F is correct *)
-    clear H1 HMatch5 HMatch3 HMatch2 HMatch4 o.
-    rewrite (mapM_grab_rep_in_messed_up_F
-             (fft_out (flatten_function_type (mf_type mf)))
-             ηss_P
-             ηss_L
-             (kc_of_fft (flatten_function_type (mf_type mf)))
-             (fft_type_vars (flatten_function_type (mf_type mf)))
-             (fft_in (flatten_function_type (mf_type mf)))
-             ρs_P
-          ) in HMatch1.
-    (* the lemma: grab_rep_correct *)
-    set (F := {|
-           fc_return := fft_out (flatten_function_type (mf_type mf));
-           fc_locals := ηss_P ++ ηss_L;
-           fc_labels := [];
-           fc_kind_ctx := kc_of_fft (flatten_function_type (mf_type mf));
-           fc_type_vars := fft_type_vars (flatten_function_type (mf_type mf))
-         |}) in *.
-    set (ϕ_in := fft_in (flatten_function_type (mf_type mf)) ) in *.
-    (* now it's just a grab_rep has_rep situation through a mapM *)
-    generalize dependent ρs_P.
-    induction ϕ_in as [|ϕ1 ϕ_inrest]; intros.
-    + cbn in HMatch1. inversion HMatch1.
-      by apply Forall2_nil.
-    + cbn in HMatch1.
-      apply bind_Some in HMatch1.
-      destruct HMatch1 as [ρ1 [Hϕ1_ρ1 Hrest]].
-      apply bind_Some in Hrest.
-      destruct Hrest as [ρ_rest [H1 H2]].
-      apply IHϕ_inrest in H1.
-      inversion H2.
-      apply Forall2_cons; split; auto.
-      apply grab_rep_correct; auto.
-  - (* foldr *) admit.
-  - apply have_instruction_type_checker_correct in H1.
-    auto.
 Admitted.
-
 
 
 Definition has_module_type_checker (m:module) (mt:module_type) : type_checker_res :=
